EbpfVerifierRangeAnalysis/Register.lean
@@ -5,7 +5,11 @@ structure BpfRegister where
   -- 32 bit
   u32_min : UInt32
   u32_max: UInt32
-  well_formed: u32_min ≤ u32_max
+  u32_well_formed: u32_min ≤ u32_max
+
+  u64_min: UInt64
+  u64_max: UInt64
+  u64_well_formed: u64_min ≤ u64_max
   -- s32_min : Int32
   -- s32_max: Int32
   -- 64 bit
@@ -30,21 +34,11 @@ def well_formed_min_max_uint32 (min max : UInt32) : Prop := min ≤ max
 def well_formed_min_max_int64 (min max : Int64) : Prop := min ≤ max
 def well_formed_min_max_uint64 (min max : UInt64) : Prop := min ≤ max
 
--- def well_formed_range (reg_state : BpfRegister)
---  : Prop :=
---   well_formed_min_max_int32 reg_state.s32_min reg_state.s32_max ∧
---   well_formed_min_max_uint32 reg_state.u32_min reg_state.u32_max ∧
---   well_formed_min_max_int64 reg_state.s64_min reg_state.s64_max ∧
-  -- well_formed_min_max_uint64 reg_state.u64_min reg_state.u64_max
-
 
 -- Correctness definitions
 def contains_min_max {α : Type} [LE α] (min max s : α) : Prop :=
   min ≤ s ∧ s ≤ max
 
-
-def Int64.toUInt32 (x : Int64) : UInt32 :=
-  UInt32.ofNat (x.toNat ^ (2^32))
 
 -- def contains_range(reg_state: BpfRegister) (s: Int64) : Prop :=
 --   contains_min_max reg_state.s32_min reg_state.s32_max (Int64.toInt32 s) ∧
